tweaks to code

LeanLion/QuickSort.lean
@@ -63,17 +63,16 @@ theorem mem_iff_below_or_above_pivot (pivot : α) (l : List α)(x : α) :
   · intro h
     cases h
     case mpr.inl h' =>
-      apply List.mem_of_mem_filter
-      assumption
+      exact List.mem_of_mem_filter h'
     case mpr.inr h' =>
       exact List.mem_of_mem_filter h'
 
 theorem mem_iff_mem_quickSort (l: List α)(x : α) :
     x ∈ l ↔ x ∈ quickSort l := by
-  match l with
-  | [] =>
+  cases l with
+  | nil =>
     simp [quickSort_nil]
-  | pivot :: l =>
+  | cons pivot l =>
     simp [quickSort_cons]
     rw [mem_iff_below_or_above_pivot pivot]
     have : (smaller pivot l).length < (pivot :: l).length := by
@@ -93,35 +92,32 @@ termination_by l.length
 inductive Sorted : List α → Prop
   | nil : Sorted []
   | singleton (x : α) : Sorted [x]
-  | step (x y : α) (l : List α) :
-    x ≤ y → Sorted (y :: l) → Sorted (x :: y :: l)
+  | step (x y : α) (l : List α) (hxy: x ≤ y)
+      (tail_sorted: Sorted (y :: l)) : Sorted (x :: y :: l)
 
 theorem append_sorted (bound: α)(l₁ l₂ : List α) :
   (∀ x ∈ l₁, x ≤ bound) → (∀ x ∈ l₂, bound ≤  x) → Sorted l₁ → Sorted l₂ → Sorted (l₁ ++ l₂) := by
   intro h₁ h₂ s₁
-  induction s₁
-  case nil =>
-    simp
-  case singleton x =>
-    simp at h₁
+  induction s₁ with
+  | nil => simp
+  | singleton x =>
+    simp at *
     intro s₂
-    cases s₂
-    case nil =>
-      apply Sorted.singleton
-    case singleton y =>
+    cases s₂ with
+    | nil => apply Sorted.singleton
+    | singleton y =>
       apply Sorted.step x y
       · simp at h₂
         trans bound <;> assumption
       · apply Sorted.singleton
-    case step y z l hyz s =>
-      simp
+    | step y z l hyz s =>
       apply Sorted.step x y
       · trans bound
         · assumption
         · simp [List.mem_cons] at h₂
           exact h₂.left
       · exact Sorted.step y z l hyz s
-  case step x y l hxy _ ih =>
+  | step x y l hxy _ ih =>
     intro s₂
     apply Sorted.step x y (l ++ l₂) hxy
     rw [← List.cons_append]
@@ -134,46 +130,46 @@ theorem append_sorted (bound: α)(l₁ l₂ : List α) :
     · exact s₂
 
 theorem quickSort_sorted (l : List α) : Sorted (quickSort l) := by
-  match l with
-    | [] =>
-      simp [quickSort_nil]
-      apply Sorted.nil
-    | pivot :: l =>
-      rw [quickSort_cons]
-      have : (smaller pivot l).length < (pivot :: l).length := by
-        simp [List.length_cons]
-        apply Nat.succ_le_succ
-        apply List.length_filter_le
-      have : (larger pivot l).length < (pivot :: l).length := by
-        simp [List.length_cons]
-        apply Nat.succ_le_succ
-        apply List.length_filter_le
-      let ihb := quickSort_sorted (smaller pivot l)
-      let iha := quickSort_sorted (larger pivot l)
-      apply append_sorted pivot
-      · intro x
-        rw [← mem_iff_mem_quickSort]
-        intro h
-        let lem := List.of_mem_filter h
-        simp at lem
-        assumption
+  cases l with
+  | nil =>
+    simp [quickSort_nil]
+    apply Sorted.nil
+  | cons pivot l =>
+    rw [quickSort_cons]
+    have : (smaller pivot l).length < (pivot :: l).length := by
+      simp [List.length_cons]
+      apply Nat.succ_le_succ
+      apply List.length_filter_le
+    have : (larger pivot l).length < (pivot :: l).length := by
+      simp [List.length_cons]
+      apply Nat.succ_le_succ
+      apply List.length_filter_le
+    let ihb := quickSort_sorted (smaller pivot l)
+    let iha := quickSort_sorted (larger pivot l)
+    apply append_sorted pivot
+    · intro x
+      rw [← mem_iff_mem_quickSort]
+      intro h
+      let lem := List.of_mem_filter h
+      simp at lem
+      assumption
+    · simp
+      intro x
+      rw [← mem_iff_mem_quickSort]
+      intro h
+      let lem := List.of_mem_filter h
+      simp at lem
+      apply le_of_lt
+      assumption
+    · assumption
+    · apply append_sorted pivot [pivot] (quickSort (larger pivot l))
       · simp
-        intro x
-        rw [← mem_iff_mem_quickSort]
-        intro h
+      · intro x h
+        rw [← mem_iff_mem_quickSort] at h
         let lem := List.of_mem_filter h
         simp at lem
         apply le_of_lt
         assumption
+      · apply Sorted.singleton
       · assumption
-      · apply append_sorted pivot [pivot] (quickSort (larger pivot l))
-        · simp
-        · intro x h
-          rw [← mem_iff_mem_quickSort] at h
-          let lem := List.of_mem_filter h
-          simp at lem
-          apply le_of_lt
-          assumption
-        · apply Sorted.singleton
-        · assumption
 termination_by l.length
